wp_safety + some progress on denotsem

theories/gitree/reify.v
@@ -25,12 +25,12 @@ Section reifiers.
   Implicit Type op : opid F.
   Implicit Type α β : IT.
 
-  Class CtxIndep (X : ofe) `{!Cofe X} (op : opid F) := {
-      cont_irrelev :
-      (∃ f : (prodO (Ins (sReifier_ops r _) ♯ X) ((sReifier_state r) ♯ X)) -n>
-               optionO (prodO (Outs (sReifier_ops r _) ♯ X) (sReifier_state r ♯ X)),
-         ∀ i σ κ, @sReifier_re _ X _ op (i, σ, κ) ≡ fmap (prodO_map κ idfun) (f (i, σ)));
-    }.
+  (* Class CtxIndep (X : ofe) `{!Cofe X} (op : opid F) := { *)
+  (*     cont_irrelev : *)
+  (*     (∃ f : (prodO (Ins (sReifier_ops r _) ♯ X) ((sReifier_state r) ♯ X)) -n> *)
+  (*              optionO (prodO (Outs (sReifier_ops r _) ♯ X) (sReifier_state r ♯ X)), *)
+  (*        ∀ i σ κ, @sReifier_re _ X _ op (i, σ, κ) ≡ fmap (prodO_map κ idfun) (f (i, σ))); *)
+  (*   }. *)
 
   Notation stateM := ((stateF ♯ IT -n> (stateF ♯ IT) * IT)).
   #[local] Instance stateT_inhab : Inhabited stateM.
@@ -229,9 +229,8 @@ Section reifiers.
     - reflexivity.
   Qed.
 
-  (* true only for ctx-independent effects *)
-  Lemma reify_vis_cont op i k1 k2 σ1 σ2 β
-    {PROP : bi} `{!BiInternalEq PROP} `{H : !(@CtxIndep IT _ op)} :
+  Lemma reify_vis_cont op i k1 (k2 : IT -n> IT) σ1 σ2 β
+    {PROP : bi} `{!BiInternalEq PROP} (* (H : IT_hom k2) *) :
     (reify (Vis op i k1) σ1 ≡ (σ2, Tick β) ⊢
      reify (Vis op i (laterO_map k2 ◎ k1)) σ1 ≡ (σ2, Tick (k2 β)) : PROP)%I.
   Proof.
@@ -240,125 +239,104 @@ Section reifiers.
       iIntros "Hr". iExFalso.
       iPoseProof (prod_equivI with "Hr") as "[_ Hk]".
       simpl. iApply (IT_tick_err_ne). by iApply internal_eq_sym.
-    - destruct H as [[f H]].
-      pose proof (H i σ1 k1) as H1.
-      pose proof (H i σ1 (laterO_map k2 ◎ k1)) as H2.
-      assert (∃ o σ', f (i, σ1) = Some (o, σ')) as [o' [σ' H3]].
-      {
-        destruct (f (i, σ1)) as [[? ?] | ?]; first (do 2 eexists; reflexivity).
-        simpl in H1. rewrite Hre in H1; inversion H1.
-      }
-      rewrite H3 in H1.
-      simpl in H1.
-      rewrite H3 in H2.
-      simpl in H2.
-      clear f H H3 Hre.
+    - (* destruct H as [[f H]]. *)
+      (* pose proof (H i σ1 k1) as H1. *)
+      (* pose proof (H i σ1 (laterO_map k2 ◎ k1)) as H2. *)
+      (* assert (∃ o σ', f (i, σ1) = Some (o, σ')) as [o' [σ' H3]]. *)
+      (* { *)
+      (*   destruct (f (i, σ1)) as [[? ?] | ?]; first (do 2 eexists; reflexivity). *)
+      (*   simpl in H1. rewrite Hre in H1; inversion H1. *)
+      (* } *)
+      (* rewrite H3 in H1. *)
+      (* simpl in H1. *)
+      (* rewrite H3 in H2. *)
+      (* simpl in H2. *)
+      (* clear f H H3 Hre. *)
       rewrite reify_vis_eq; last first.
-      { by rewrite H1. }
-      rewrite reify_vis_eq; last first.
-      { by rewrite H2. }
+      { by rewrite Hre. }
       iIntros "Hr".
       iPoseProof (prod_equivI with "Hr") as "[Hs Hk]".
-      iApply prod_equivI. simpl. iSplit; eauto.
       iPoseProof (Tau_inj' with "Hk") as "Hk".
-      iApply Tau_inj'. iRewrite "Hk".
-      rewrite laterO_map_Next. done.
-  Qed.
-
-  Lemma reify_input_cont_inv op i (k1 : _ -n> laterO IT) (k2 : IT -n> IT) σ1 σ2 β
-    {PROP : bi} `{!BiInternalEq PROP} `{H : !(@CtxIndep IT _ op)} :
-    (reify (Vis op i (laterO_map k2 ◎ k1)) σ1 ≡ (σ2, Tick β)
-     ⊢ ∃ α, reify (Vis op i k1) σ1 ≡ (σ2, Tick α) ∧ ▷ (β ≡ k2 α)
-      : PROP)%I.
-  Proof.
-    destruct (sReifier_re r op (i, σ1, (laterO_map k2 ◎ k1))) as [[o σ2']|] eqn:Hre; last first.
-    - rewrite reify_vis_None; last by rewrite Hre//.
-      iIntros "Hr". iExFalso.
-      iPoseProof (prod_equivI with "Hr") as "[_ Hk]".
-      simpl. iApply (IT_tick_err_ne). by iApply internal_eq_sym.
-    - rewrite reify_vis_eq; last first.
-      { by rewrite Hre. }
-      iIntros "Hr". simpl.
-      iPoseProof (prod_equivI with "Hr") as "[#Hs #Hk]".
       simpl.
-      iPoseProof (Tau_inj' with "Hk") as "Hk'".
-      destruct H as [[f H]].
-      pose proof (H i σ1 k1) as H1.
-      pose proof (H i σ1 (laterO_map k2 ◎ k1)) as H2.
-      assert (∃ o, f (i, σ1) ≡ Some (o, σ2')) as [o' H3].
-      {
-        destruct (f (i, σ1)) as [[? ?] | ?].
-        - simpl in H2.
-          rewrite Hre in H2.
-          inversion H2 as [? ? H2' |]; subst; inversion H2'; simpl in *; subst.
-          eexists _; do 2 f_equiv; first reflexivity; symmetry; assumption.
-        - simpl in H2.
-          rewrite Hre in H2.
-          inversion H2.
-      }
-      rewrite H3 in H1.
-      simpl in H1.
-      rewrite H3 in H2.
-      simpl in H2.
-      destruct (Next_uninj (k1 o')) as [a Hk1].
-      iExists (a).
-      rewrite reify_vis_eq; last first.
-      { by rewrite H1. }
-      iSplit.
-      + iApply prod_equivI. simpl. iSplit; eauto.
-        iApply Tau_inj'. done.
-      + iAssert (laterO_map k2 (Next a) ≡ Next β)%I as "Ha".
-        {
-          iSimpl in "Hk'". iRewrite -"Hk'".
-          iPureIntro. rewrite -Hk1.
-          rewrite Hre in H2.
-          inversion H2 as [? ? H2' |]; subst; inversion H2'; simpl in *; subst.
-          symmetry; assumption.
-        }
-        iAssert (Next (k2 a) ≡ Next β)%I as "Hb".
-        { iRewrite -"Ha". iPureIntro.
-          rewrite laterO_map_Next. done. }
-        iNext. by iApply internal_eq_sym.
-  Qed.
+      (* pose proof hom_vis. *)
+      (* rewrite H.       *)
+      (* iRewrite - "Hs". *)
+      (* rewrite reify_vis_eq; last first. *)
+      (* { by rewrite Hre. } *)
+      (* iRewrite "Hk". *)
+      (* rewrite -Tick_eq. *)
+      (* done. *)
+      (* reflexivity. *)
+      (* rewrite term *)
+      (* iApply prod_equivI. simpl.       *)
+      (* iSplit; eauto. *)
+      (* iApply Tau_inj'. iRewrite "Hk". *)
+      (* rewrite laterO_map_Next. done. *)
+  Admitted.
 
-  Lemma reify_is_always_a_tick op x k σ β σ' `{H : !(@CtxIndep IT _ op)} :
+  (* Lemma reify_input_cont_inv op i (k1 : _ -n> laterO IT) (k2 : IT -n> IT) σ1 σ2 β *)
+  (*   {PROP : bi} `{!BiInternalEq PROP} *)
+  (*   (g : (IT -n> IT) -n> (prodO (stateF ♯ IT) IT) -n> (prodO (stateF ♯ IT) IT)) *)
+  (*   (H : reify (Vis op i (laterO_map k2 ◎ k1)) σ1 ≡ (g k2) (reify (Vis op i k1) σ1)) *)
+  (*   : *)
+  (*   (reify (Vis op i (laterO_map k2 ◎ k1)) σ1 ≡ (σ2, Tick β) *)
+  (*    ⊢ ∃ α, reify (Vis op i k1) σ1 ≡ (σ2, Tick α) ∧ ▷ (β ≡ k2 α) *)
+  (*     : PROP)%I. *)
+  (* Proof. *)
+  (*   destruct (sReifier_re r op (i, σ1, (laterO_map k2 ◎ k1))) as [[o σ2']|] eqn:Hre; last first. *)
+  (*   - rewrite reify_vis_None; last by rewrite Hre//. *)
+  (*     iIntros "Hr". iExFalso. *)
+  (*     iPoseProof (prod_equivI with "Hr") as "[_ Hk]". *)
+  (*     simpl. iApply (IT_tick_err_ne). by iApply internal_eq_sym. *)
+  (*   - rewrite reify_vis_eq; last first. *)
+  (*     { by rewrite Hre. } *)
+  (*     iIntros "Hr". simpl. *)
+  (*     iPoseProof (prod_equivI with "Hr") as "[#Hs #Hk]". *)
+  (*     simpl. *)
+  (*     iPoseProof (Tau_inj' with "Hk") as "Hk'".       *)
+  (*     destruct (Next_uninj o) as [a Hk1]. *)
+  (*     iExists (a). *)
+  (*     assert (Hre' : sReifier_re r op (i, σ1, laterO_map k2 ◎ k1) ≡ Some (o, σ2')). *)
+  (*     { by rewrite Hre. } *)
+  (*     apply reify_vis_eq in Hre'. *)
+  (*     rewrite Hre' in H. *)
+  (*     rewrite H. *)
+  (*     iRewrite - "Hr". *)
+  (*     epose proof (reify_vis_eq _ _ _ _ _ _ Hre). *)
+  (*     rewrite reify_vis_eq; last first. *)
+  (*     { by rewrite H1. } *)
+  (*     iSplit. *)
+  (*     + iApply prod_equivI. simpl. iSplit; eauto. *)
+  (*       iApply Tau_inj'. done. *)
+  (*     + iAssert (laterO_map k2 (Next a) ≡ Next β)%I as "Ha". *)
+  (*       { *)
+  (*         iSimpl in "Hk'". iRewrite -"Hk'". *)
+  (*         iPureIntro. rewrite -Hk1. *)
+  (*         rewrite Hre in H2. *)
+  (*         inversion H2 as [? ? H2' |]; subst; inversion H2'; simpl in *; subst. *)
+  (*         symmetry; assumption. *)
+  (*       } *)
+  (*       iAssert (Next (k2 a) ≡ Next β)%I as "Hb". *)
+  (*       { iRewrite -"Ha". iPureIntro. *)
+  (*         rewrite laterO_map_Next. done. } *)
+  (*       iNext. by iApply internal_eq_sym. *)
+  (* Qed. *)
+
+  Lemma reify_is_always_a_tick op x k σ β σ' :
     reify (Vis op x k) σ ≡ (σ', β) → (∃ β', β ≡ Tick β') ∨ (β ≡ Err RuntimeErr).
   Proof.
     destruct (sReifier_re r op (x, σ, k)) as [[o σ'']|] eqn:Hre; last first.
     - rewrite reify_vis_None; last by rewrite Hre//.
       intros [_ ?]. by right.
-    - destruct H as [[f H]].
-      specialize (H x σ k).
-      rewrite reify_vis_eq; last by rewrite Hre.
+    - rewrite reify_vis_eq;last by rewrite Hre.
       intros [? Ho].
+      left.
       simpl in *.
-      assert (∃ o, f (x, σ) ≡ Some (o, σ'')) as [o' H'].
-      {
-        destruct (f (x, σ)) as [[? ?] | ?].
-        - simpl in H.
-          rewrite Hre in H.
-          inversion H as [? ? H' |]; subst; inversion H'; simpl in *; subst.
-          eexists _; do 2 f_equiv; first reflexivity; symmetry; assumption.
-        - simpl in H.
-          rewrite Hre in H.
-          inversion H.
-      }
-      assert (H'' : sReifier_re r op (x, σ, k) ≡ (prodO_map k idfun) <$> (Some (o', σ''))).
-      {
-        rewrite H.
-        f_equiv.
-        - intros ???; simpl.
-          solve_proper.
-        - assumption.
-      }
-      simpl in H''.
-      rewrite Hre in H''.
-      inversion H'' as [? ? H''' |]; subst; inversion H''' as [H1 ?]; simpl in *; subst.
-      rewrite <-!Ho, H1.
-      destruct (Next_uninj (k o')) as [lβ Hlb].
-      left. exists (lβ).
-      rewrite Tick_eq.
-      rewrite -Hlb. symmetry. rewrite -H1. apply Ho.
+      destruct (Next_uninj o) as [t Ht].
+      exists (t).
+      rewrite <-Ho.
+      rewrite Ht.
+      reflexivity.
   Qed.
 
 End reifiers.
